solve Exercise 4.2

HelloTypeSystem/ML2.lean
@@ -7,7 +7,19 @@ namespace HelloTypeSystem
 \[基礎概念,4章]
 -/
 namespace ML2
-open HelloTypeSystem.ML1 (Value Error Result)
+open HelloTypeSystem.ML1 (Value)
+
+abbrev Error := Unit
+private def error : Error := ()
+
+abbrev Result := Error ⊕ Value
+
+instance : OfNat Result n where
+  ofNat := .inr (.Z n)
+instance : Coe Value Result where
+  coe := .inr
+instance : Coe Error Result where
+  coe := .inl
 
 /--
 変数名
@@ -44,7 +56,6 @@ instance : Sub Expr where
   sub := Expr.Sub
 instance : Mul Expr where
   mul := Expr.Mul
-notation e₁ " < " e₂ => Expr.LT e₁ e₂
 notation e₁ " ? " e₂ " : " e₃ => Expr.If e₁ e₂ e₃
 notation "LET " x:max " = " e₁ " IN " e₂ => Expr.Let x e₁ e₂
 
@@ -74,13 +85,155 @@ inductive Evaluation : Env → Expr → Result → Type
     : Evaluation E (e₁ - e₂) i₃
   | Mul {i₁ i₂ i₃: Int} (d₁ : Evaluation E e₁ i₁) (d₂ : Evaluation E e₂ i₂) (h : i₁ * i₂ = i₃ := by trivial)
     : Evaluation E (e₁ * e₂) i₃
-  | LTT {i₁ i₂ i₃: Int} (d₁ : Evaluation E e₁ i₁) (d₂ : Evaluation E e₂ i₂) (h : i₁ < i₂ := by trivial)
-    : Evaluation E (e₁ < e₂) true
-  | LTF {i₁ i₂ i₃: Int} (d₁ : Evaluation E e₁ i₁) (d₂ : Evaluation E e₂ i₂) (h : ¬ i₁ < i₂ := by trivial)
-    : Evaluation E (e₁ < e₂) false
+  | LTT {i₁ i₂: Int} (d₁ : Evaluation E e₁ i₁) (d₂ : Evaluation E e₂ i₂) (h : i₁ < i₂ := by trivial)
+    : Evaluation E (.LT e₁ e₂) true
+  | LTF {i₁ i₂: Int} (d₁ : Evaluation E e₁ i₁) (d₂ : Evaluation E e₂ i₂) (h : ¬ i₁ < i₂ := by trivial)
+    : Evaluation E (.LT e₁ e₂) false
   | IfT {v₂ : Value} (dc : Evaluation E e₁ true) (dt : Evaluation E e₂ v₂)
     : Evaluation E (e₁ ? e₂ : e₃) v₂
   | IfF {v₃ : Value} (dc : Evaluation E e₁ false) (df : Evaluation E e₃ v₃)
     : Evaluation E (e₁ ? e₂ : e₃) v₃
   | Let {v₁ v₂ : Value} (d₁ : Evaluation E e₁ v₁) (d₂ : Evaluation ((x, v₁) :: E) e₂ v₂)
     : Evaluation E (LET x = e₁ IN e₂) v₂
+
+  | VarUnbound {x : Var}
+    : Evaluation [] x error
+  | VarErr {x : Var}
+    : Evaluation E x (.inl ε)
+
+  | AddBoolL (d : Evaluation E e (.inr (.B b)))
+    : Evaluation E (e + _) error
+  | AddBoolR (d : Evaluation E e (.inr (.B b)))
+    : Evaluation E (_ + e) error
+  | AddErrL (d : Evaluation E e (.inl ε))
+    : Evaluation E (e + _) ε
+  | AddErrR (d : Evaluation E e (.inl ε))
+    : Evaluation E (_ + e) ε
+
+  | SubBoolL (d : Evaluation E e (.inr (.B b)))
+    : Evaluation E (e - _) error
+  | SubBoolR (d : Evaluation E e (.inr (.B b)))
+    : Evaluation E (_ - e) error
+  | SubErrL (d : Evaluation E e (.inl ε))
+    : Evaluation E (e - _) ε
+  | SubErrR (d : Evaluation E e (.inl ε))
+    : Evaluation E (_ - e) ε
+
+  | MulBoolL (d : Evaluation E e (.inr (.B b)))
+    : Evaluation E (e * _) error
+  | MulBoolR (d : Evaluation E e (.inr (.B b)))
+    : Evaluation E (_ * e) error
+  | MulErrL (d : Evaluation E e (.inl ε))
+    : Evaluation E (e * _) ε
+  | MulErrR (d : Evaluation E e (.inl ε))
+    : Evaluation E (_ * e) ε
+
+  | LTBoolL (d : Evaluation E e (.inr (.B b)))
+    : Evaluation E (.LT e _) error
+  | LTBoolR (d : Evaluation E e (.inr (.B b)))
+    : Evaluation E (.LT _ e) error
+  | LTErrL (d : Evaluation E e (.inl ε))
+    : Evaluation E (.LT e _) ε
+  | LTErrR (d : Evaluation E e (.inl ε))
+    : Evaluation E (.LT _ e) ε
+
+  | IfInt (d : Evaluation E e (.inr (.Z i)))
+    : Evaluation E (.If e _ _) error
+  | IfErr (d : Evaluation E e (.inl ε))
+    : Evaluation E (.If e _ _) ε
+  | IfTErr {ε₂ : Error} (dc : Evaluation E e₁ true) (dt : Evaluation E e₂ ε₂)
+    : Evaluation E (e₁ ? e₂ : e₃) ε₂
+  | IfFErr {ε₃ : Error} (dc : Evaluation E e₁ false) (df : Evaluation E e₃ ε₃)
+    : Evaluation E (e₁ ? e₂ : e₃) ε₃
+
+  | LetBindingErr {ε₁ : Error} (d₁ : Evaluation E e₁ ε₁)
+    : Evaluation E (LET x = e₁ IN _) ε₁
+  | LetExprErr {v₁ : Value} {ε₂ : Error} (d₁ : Evaluation E e₁ v₁) (d₂ : Evaluation ((x, v₁) :: E) e₂ ε₂)
+    : Evaluation E (LET x = e₁ IN e₂) ε₂
+
+private def Expr.eval_aux (expr : Expr) (env : Env) : (r : Result) × (Evaluation env expr r) :=
+  match expr with
+  | Lit v =>
+      match v with
+      | .Z i => ⟨i, .Int⟩
+      | .B b => ⟨b, .Bool⟩
+  | Var x =>
+      match env with
+      | [] => ⟨error, .VarUnbound⟩
+      | ⟨y, v⟩ :: env' =>
+          if h : y = x then
+            ⟨v, h ▸ .Var⟩
+          else
+            let ⟨r, d⟩ := Expr.eval_aux (Var x) env'
+            match r with
+            | .inr v => ⟨v, .VarIr d h⟩
+            | .inl ε => ⟨ε, .VarErr⟩
+  | Add e₁ e₂ =>
+      let ⟨r₁, d₁⟩ := e₁.eval_aux env
+      let ⟨r₂, d₂⟩ := e₂.eval_aux env
+      match r₁, r₂ with
+      | .inr (.Z i₁), .inr (.Z i₂) => ⟨i₁ + i₂, .Add d₁ d₂⟩
+      | .inr (.B b₁), _            => ⟨error,   .AddBoolL d₁⟩
+      | .inl ε₁,      _            => ⟨ε₁,      .AddErrL d₁⟩
+      | _,            .inr (.B b₂) => ⟨error,   .AddBoolR d₂⟩
+      | _,            .inl ε₂      => ⟨ε₂,      .AddErrR d₂⟩
+  | Sub e₁ e₂ =>
+      let ⟨r₁, d₁⟩ := e₁.eval_aux env
+      let ⟨r₂, d₂⟩ := e₂.eval_aux env
+      match r₁, r₂ with
+      | .inr (.Z i₁), .inr (.Z i₂) => ⟨i₁ - i₂, .Sub d₁ d₂⟩
+      | .inr (.B b₁), _            => ⟨error,   .SubBoolL d₁⟩
+      | .inl ε₁,      _            => ⟨ε₁,      .SubErrL d₁⟩
+      | _,            .inr (.B b₂) => ⟨error,   .SubBoolR d₂⟩
+      | _,            .inl ε₂      => ⟨ε₂,      .SubErrR d₂⟩
+  | Mul e₁ e₂ =>
+      let ⟨r₁, d₁⟩ := e₁.eval_aux env
+      let ⟨r₂, d₂⟩ := e₂.eval_aux env
+      match r₁, r₂ with
+      | .inr (.Z i₁), .inr (.Z i₂) => ⟨i₁ * i₂, .Mul d₁ d₂⟩
+      | .inr (.B b₁), _            => ⟨error,   .MulBoolL d₁⟩
+      | .inl ε₁,      _            => ⟨ε₁,      .MulErrL d₁⟩
+      | _,            .inr (.B b₂) => ⟨error,   .MulBoolR d₂⟩
+      | _,            .inl ε₂      => ⟨ε₂,      .MulErrR d₂⟩
+  | LT e₁ e₂ =>
+      let ⟨r₁, d₁⟩ := e₁.eval_aux env
+      let ⟨r₂, d₂⟩ := e₂.eval_aux env
+      match r₁, r₂ with
+      | .inr (.Z i₁), .inr (.Z i₂) =>
+          if h : i₁ < i₂ then
+            ⟨true, .LTT d₁ d₂ h⟩
+          else
+            ⟨false, .LTF d₁ d₂ h⟩
+      | .inr (.B b₁), _            => ⟨error, .LTBoolL d₁⟩
+      | .inl ε₁,      _            => ⟨ε₁,    .LTErrL d₁⟩
+      | _,            .inr (.B b₂) => ⟨error, .LTBoolR d₂⟩
+      | _,            .inl ε₂      => ⟨ε₂,    .LTErrR d₂⟩
+  | If e₁ e₂ e₃ =>
+      let ⟨r₁, d₁⟩ := e₁.eval_aux env
+      match r₁ with
+      | .inr (.B true) =>
+          let ⟨r₂, d₂⟩ := e₂.eval_aux env
+          match r₂ with
+          | .inr v => ⟨v, .IfT d₁ d₂⟩
+          | .inl ε => ⟨ε, .IfTErr d₁ d₂⟩
+      | .inr (.B false) =>
+          let ⟨r₃, d₃⟩ := e₃.eval_aux env
+          match r₃ with
+          | .inr v => ⟨v, .IfF d₁ d₃⟩
+          | .inl ε => ⟨ε, .IfFErr d₁ d₃⟩
+      | .inr (.Z _) => ⟨error, .IfInt d₁⟩
+      | .inl ε => ⟨ε, .IfErr d₁⟩
+  | Let x e₁ e₂ =>
+      let ⟨r₁, d₁⟩ := e₁.eval_aux env
+      match r₁ with
+      | .inr v =>
+          let ⟨r₂, d₂⟩ := e₂.eval_aux ((x, v) :: env)
+          match r₂ with
+          | .inr v => ⟨v, .Let d₁ d₂⟩
+          | .inl ε => ⟨ε, .LetExprErr d₁ d₂⟩
+      | .inl ε => ⟨ε, .LetBindingErr d₁⟩
+
+/--
+`eval`はML2式`e`を評価してその結果を返します。
+-/
+def Expr.eval (e : Expr) : Result := (e.eval_aux []).fst
